Define lookup

syntax.sig
@@ -5,7 +5,7 @@ Ki : Type
 TmAbs : (bind Tm in Tm) -> Tm
 TmApp : Tm -> Tm -> Tm
 
-TyAbs : (bind Ty in Ty) -> Ty
+TyAbs : Ki -> (bind Ty in Ty) -> Ty
 TyApp : Ty -> Ty -> Ty
 TyForall : Ki -> (bind Ty in Ty) -> Ty
 TyFun : Ty -> Ty -> Ty
